@@ -1,0 +1,10 @@
+/-
+`uartinit`'s interface, instantiated from its proof.
+-/
+import Xv6.ProofUartinit
+
+namespace Xv6
+
+theorem Uartinit (UI : UARTINITONE) : UARTINIT := uartinit_proof UI
+
+end Xv6
